src/tls/PKI.fsti
@@ -3,8 +3,9 @@ module PKI
 // This module is implemented natively
 
 open FStar.HyperStack.ST
-open TLSConstants
-
-val init: cafile:string -> server_certs:list (string * string * bool) -> St FStar.Dyn.dyn
-val tls_callbacks: FStar.Dyn.dyn -> St cert_cb
-val free: FStar.Dyn.dyn -> St unit
+open TLS.Callbacks
+val init: 
+  cafile:string -> 
+  server_certs:list (string * string * bool) -> context
+val tls_callbacks: context -> St cert_cb
+val free: context -> St unit
