src/tls/TLS.Handshake.Machine.fst
@@ -1,0 +1,289 @@
+module TLS.Handshake.Machine
+
+/// Drafting the Handshake verified state machine, integrating
+/// refinements, monotonic properties, and stateful properties from
+/// Transcript, Negotiation, KeySchedule.
+
+open FStar.Error
+open FStar.Bytes // still used for cookies, tickets, signatures... 
+
+open Mem
+open TLSError
+open TLSInfo
+open TLSConstants
+
+module B = LowStar.Buffer
+module HS = FStar.HyperStack
+module HST = FStar.HyperStack.ST
+
+module HSM = HandshakeMessages
+module LP = LowParse.Low.Base
+module Transcript = HSL.Transcript 
+
+// let Secret = Handshake.Secret
+
+// missing indexes? both elements should be Client-specific, with
+// resumeInfo only for clients.
+let client_config = config * Negotiation.resumeInfo 
+
+// Helpful refinement within Secret?
+assume val is_psk: Idx.id -> bool 
+
+// May also depend on the resumeInfo, to be sorted out once we fix the
+// config type.
+assume val psk_ids_of_config: client_config -> list (i:Idx.id{is_psk i})
+assume val groups_of_config: client_config -> list CommonDH.group  
+
+// Offered, depending on first PSK or first ciphersuite.
+// May be overwritten by ServerHello 
+assume val ha_of_offer: Negotiation.offer -> Spec.Hash.Definitions.hash_alg
+
+// from Handshake.Secret, currently broken
+assume type secret_c13_wait_ServerHello 
+  (psks  : list (i:_{is_psk i})) 
+  (groups: list CommonDH.group)
+
+// we may need an extra ghost in the implementation of the type above.
+assume val shares_of_ks:
+  #psks  : list (i:_{is_psk i}) ->
+  #groups: list CommonDH.group -> 
+  secret_c13_wait_ServerHello psks groups -> option Extensions.keyShareClientHello
+
+// should be in transcript
+let trans (n:nat) = tr: Transcript.transcript_t { Transcript.transcript_size tr <= n }
+
+
+/// State machine for the connection handshake (private to Handshake).
+/// Each role now has its own type.
+noeq type client_state  
+  (region:rgn) // unused for now; worth the trouble? passed only as stateful-invariant argument? 
+  (cfg: client_config) 
+  (nonce: TLSInfo.random) // could be a function of the transcript, saving one argument? 
+  = 
+
+  // allocation state, initially empty
+  | C_init: 
+    client_state region cfg nonce 
+
+  // intermediate step for witnessing the truncated transcript, a
+  // pre-condition for the binder HMACs. 
+  // TODO The Transcript state should be TruncatedHello. 
+  | C_truncated_ClientHello:
+    transcript: Ghost.erased (trans 0) -> 
+    offer: Negotiation.offer (* TODO with zeroed binders *) ->
+    digest: Transcript.state (ha_of_offer offer) -> 
+    ks: secret_c13_wait_ServerHello (psk_ids_of_config cfg) (groups_of_config cfg) 
+    { let transcript = Ghost.reveal transcript in 
+      transcript == Transcript.Hello None (HSM.M_client_hello offer) /\
+      ( exists (now:UInt32.t). (Correct offer == Negotiation.client_offer (fst cfg) nonce (shares_of_ks ks) (snd cfg) now)) }
+    -> 
+    client_state region cfg nonce 
+
+  // waiting for plaintext ServerHello.
+  | C_wait_ServerHello: 
+    transcript: Ghost.erased (trans 0) -> 
+    offer: Negotiation.offer -> 
+    digest: Transcript.state (ha_of_offer offer) -> 
+    ks: secret_c13_wait_ServerHello (psk_ids_of_config cfg) (groups_of_config cfg) 
+    { let transcript = Ghost.reveal transcript in 
+      transcript == Transcript.Hello None (HSM.M_client_hello offer) /\
+      //Negotiation.correct_client_offer nego cfg nonce (shares_of_ks ks) resume now
+      ( exists (now:UInt32.t). (Correct offer == Negotiation.client_offer (fst cfg) nonce (shares_of_ks ks) (snd cfg) now))
+      } -> 
+    client_state region cfg nonce 
+
+  // TLS 1.3 waiting for encrypted handshake
+  | C13_wait_Finished1: 
+    transcript: Ghost.erased (trans 1) -> 
+    nego: Negotiation.mode ->
+    digest: Transcript.state (Negotiation.hashAlg nego) 
+    { let transcript = Ghost.reveal transcript in
+      let offer = nego.Negotiation.n_offer in (
+      exists (sh:_) (now:UInt32.t) (shares:_). 
+      Correct offer == Negotiation.client_offer (fst cfg) nonce shares (snd cfg) now /\
+      Correct nego == Negotiation.accept_ServerHello (fst cfg) offer sh /\ 
+      Transcript.nego_version (HSM.M_client_hello offer) (HSM.M_server_hello sh) == TLS_1p3 /\ 
+      transcript == Transcript.Transcript13 None (HSM.M_client_hello offer) (HSM.M_server_hello sh) [] )
+    }                                 
+    -> 
+    //i:   Secret.hs_id ->
+    //ams: Secret.ams (Secret.ams_of_hms i) ->
+    //cfk: Secret.fink (Secret.cfk_of_hms i) ->
+    //sfk: Secret.fink (Secret.sfk_of_hms i) -> 
+    client_state region cfg nonce 
+
+(* TBC. It would be nice to reach Complete with some label abstraction.
+  // TLS 1.3 #20 aggravation, optional from C13_wait_Finished1
+  | C13_sent_EOED: 
+    transcript: Ghost.erased (transcript: trans 4 { Transcript.Hello? transcript }) -> 
+    //i:   Secret.hs_id ->
+    //ams: Secret.ams (Secret.ams_of_hms i) ->
+    //cfk: Secret.fink (Secret.cfk_of_hms i) ->
+    //digest (* _EOED *) ->
+    //option HSM.cr13 -> 
+    st region role cfg resume nonce 
+
+  | C13_complete: // TLS 1.3 waiting for post-handshake messages (TBC rekeying)
+    transcript: Ghost.erased (transcript: trans 10 { Transcript.Hello? transcript }) -> 
+    // i:   Secret.ams_id ->
+//    rms: Secret.secret (rms_of_ams i tr) (* for accepting resumption tickets *) ->
+    st region role cfg resume nonce 
+
+  | C12_wait_CCS1 of digest      // TLS resume, digest to be authenticated by server
+  | C12_wait_R_Finished1 of digest // TLS resume, digest to be authenticated by server
+  | C12_wait_ServerHelloDone:
+    // cr:random ->
+    machineState
+
+  | C12_wait_CCS2: // TLS classic
+    ks: Secret.ks12_state ->
+    digest_Finished1: digest -> // to be authenticated in the server Finished
+    machineState
+
+  | C12_wait_Finished2: // TLS classic
+    ks: Secret.ks12_state ->
+    digest_Finished1: digest -> // to be authenticated in the server Finished
+    machineState
+
+  | C_Complete // TODO add state
+*)
+
+// we embed in the type above refinements for functional properties
+// and witnessed properties, but we also need a stateful invariant.
+
+let client_invariant 
+  (#region:rgn) (#cfg: client_config) (#nonce: TLSInfo.random) 
+  (state: client_state region cfg nonce)
+  (h: HS.mem) 
+= 
+  match state with 
+  | C_init -> True
+
+  | C_truncated_ClientHello transcript offer digest ks 
+  | C_wait_ServerHello transcript offer digest ks -> 
+    let transcript = Ghost.reveal transcript in 
+    Transcript.invariant digest transcript h
+    // Secret.invariant ks h
+
+  | C13_wait_Finished1 transcript mode digest ->
+    let transcript = Ghost.reveal transcript in 
+    Transcript.invariant digest transcript h
+    // Secret.invariant_C13_wait_Finished1 ks
+  | _ -> False 
+  
+
+/// We define an update condition on the state that encodes the state
+/// machine and ensures stability on selected properties of
+/// interest. For example, the transcript is monotonic; and
+/// Negotiation's offer and mode are SSA.
+
+let step
+  (#region:rgn) (#cfg: client_config) (#nonce: TLSInfo.random)
+  (st0 st1: client_state region cfg nonce)
+= 
+  match st0, st1 with 
+  | C_init,
+    C_truncated_ClientHello transcript0 offer0 digest0 ks0 -> True
+
+  | C_truncated_ClientHello transcript0 offer0 digest0 ks0,
+    C_wait_ServerHello      transcript1 offer1 digest1 ks1 ->
+    let transcript0 = Ghost.reveal transcript0 in 
+    let transcript1 = Ghost.reveal transcript1 in 
+    exists (binders:_). 
+    Some transcript1 == Transcript.transition_hsm transcript0 binders /\
+    //19-05-15 can we avoid the option? 
+    
+    True //offer1 == transcript_offer transcript1 
+
+  | C_wait_ServerHello      transcript0 offer0 digest0 ks0,
+    C13_wait_Finished1      transcript1 mode1 digest1 ->
+    let transcript0 = Ghost.reveal transcript0 in 
+    let transcript1 = Ghost.reveal transcript1 in (
+    exists (sh:_). 
+    Some transcript1 == Transcript.transition_hsm transcript0 sh )
+
+  | _, _ -> False 
+
+// sample lemma: the offer is SSA. 
+
+let st_offer
+  (#region:rgn) (#cfg: client_config) (#nonce: TLSInfo.random)
+  (st0: client_state region cfg nonce) 
+= 
+  match st0 with 
+  | C_wait_ServerHello transcript0 offer0 digest0 ks0 -> Some offer0 
+  | C13_wait_Finished1 transcript0 mode0 digest0 -> Some mode0.Negotiation.n_offer
+  | _ -> None 
+
+let m_offer 
+  (#region:rgn) (#cfg: client_config) (#nonce: TLSInfo.random)
+  (st0 st1: client_state region cfg nonce):
+  Lemma (
+    let o0 = st_offer st0 in
+    let o1 = st_offer st1 in
+    step st0 st1 /\ Some? o0 ==> o1 == o0)
+=
+  ()
+
+let mrel 
+  (#region:rgn) (#cfg: client_config) (#nonce: TLSInfo.random)
+= TC.reflexive_transitive_closure (step #region #cfg #nonce)
+
+/// Main type for the connection handshake
+noeq abstract type t 
+  (region:rgn) 
+  = 
+  | C_State: 
+  cfg: client_config ->
+  nonce: TLSInfo.random ->
+  state: HST.mreference 
+    (client_state region cfg nonce) 
+    (mrel #region #cfg #nonce) 
+    { HS.frameOf state = region } -> 
+  t region 
+
+(*
+/// Testing monotonicity; not quite there. 
+
+let witness_offer (#region:rgn) (st:t region): 
+  ST (
+    o: Negotiation.offer {
+      let C_State cfg nonce r = st in 
+      token_p r (fun h0 -> st_offer (HS.sel h0 r) = Some o) } )
+  (requires fun h0 -> 
+    let C_State cfg nonce r = st in 
+    h0 `HS.contains` r)
+  (ensures fun h0 r h1 -> True)
+= 
+  match st with 
+  | C_State cfg nonce r -> (
+    match st_offer !r with 
+      | Some o -> (
+          let p h0 = st_offer (HS.sel h0 r) == Some o in 
+          TC.inv_closure step p m_offer;
+          assert(p `HST.stable_on` r);
+          witness_p r p;
+          o )
+    | _ -> admit())
+*)
+
+
+(* TODO server-side
+  | S_Idle
+
+  | S13_sent_ServerHello:      // TLS 1.3, intermediate state to encryption
+    i: Idx.id -> // Secret.esId ->
+    idh: Idx.id_dhe ->
+    ks: Secret.s13_wait_ServerHello i idh -> machineState
+
+
+  | S_wait_EOED                // Waiting for EOED
+  | S_wait_Finished2 of digest // TLS 1.3, digest to be MACed by client
+  | S_wait_CCS1                // TLS classic
+  | S_wait_Finished1 of digest // TLS classic, digest to the MACed by client
+  | S_wait_CCS2 of digest      // TLS resume (CCS)
+  | S_wait_CF2 of digest       // TLS resume (CF)
+  | S_Complete
+*) 
+
+
